fx

Logic/Modal/Standard/Kripke/KH.lean
@@ -2,84 +2,53 @@ import Logic.Modal.Standard.Kripke.GL.Completeness
 
 namespace LO.Modal.Standard
 
-variable [DecidableEq α]
+variable [DecidableEq α] [Inhabited α]
 
+-- TODO: 結局使わなかった．
 namespace Formula
 
-@[simp] lemma complexity_not (p : Formula α) : p.complexity < (~p).complexity := by simp [Formula.complexity]
-
-abbrev UniformSubstitution (α) := α → Formula α
-
-def subst (p : Formula α) (σ : UniformSubstitution α) : Formula α :=
-  match p with
-  | ⊥ => ⊥
-  | ⊤ => ⊤
-  | atom b => σ b
-  | ~p => ~(p.subst σ)
-  | p ⋏ q => (p.subst σ) ⋏ (q.subst σ)
-  | p ⋎ q => (p.subst σ) ⋎ (q.subst σ)
-  | p ⟶ q => (p.subst σ)  ⟶ (q.subst σ)
-  | box p => □(p.subst σ)
-
-def subst₂ (p : Formula α) (a : α) (t : Formula α) : Formula α :=
+def subst (p : Formula α) (a : α) (t : Formula α) : Formula α :=
   match p with
   | ⊥ => ⊥
   | ⊤ => ⊤
   | atom b => if b = a then t else atom b
-  | ~p => ~(p.subst₂ a t)
-  | p ⋏ q => (p.subst₂ a t) ⋏ (q.subst₂ a t)
-  | p ⋎ q => (p.subst₂ a t) ⋎ (q.subst₂ a t)
-  | p ⟶ q => (p.subst₂ a t)  ⟶ (q.subst₂ a t)
-  | box p => □(p.subst₂ a t)
-
-lemma Kripke.Satisfies.subst_closed {p : Formula α} {M : Kripke.Model α} {x : M.World} (a : α) (t : Formula α) : x ⊧ p → x ⊧ (p.subst₂ a t) := by
-  induction p using Formula.rec' generalizing x with
-  | hatom b =>
-    simp [Formula.subst₂];
-    by_cases h : b = a;
-    . simp_all;
-      sorry;
-    . simp_all;
-  | hverum =>
-    simp [Formula.subst₂];
-  | hfalsum => simp_all [Formula.subst₂];
-  | hneg p ih =>
-    simp [Formula.subst₂];
-    sorry;
-  | hand p q ihp ihq => simp_all [Formula.subst₂];
-  | hor p q ihp ihq =>
-    rintro (hp | hq);
-    . left; exact ihp hp;
-    . right; exact ihq hq;
-  | himp p q ihp ihq =>
-    simp [Formula.subst₂];
-    rintro hp hq;
-    sorry;
-  | hbox p ih =>
-    simp [Formula.subst₂];
-    intro h y Rxy;
-    apply ih $ @h y Rxy;
+  | ~p => ~(p.subst a t)
+  | p ⋏ q => (p.subst a t) ⋏ (q.subst a t)
+  | p ⋎ q => (p.subst a t) ⋎ (q.subst a t)
+  | p ⟶ q => (p.subst a t)  ⟶ (q.subst a t)
+  | box p => □(p.subst a t)
 
 end Formula
 
--- MEMO: `Ax(Λ)`がきちんと公理図式として要請を満たせば`hMaxm`の証明は一般化できる
-lemma GL_deduct_substitution {p : Formula α} (a : α) (q : Formula α) : 𝐆𝐋 ⊢! p → 𝐆𝐋 ⊢! (p.subst₂ a q) := by
+lemma GL_deduct_substitution {p : Formula α} (a : α) (q : Formula α) : 𝐆𝐋 ⊢! p → 𝐆𝐋 ⊢! (p.subst a q) := by
   intro h;
   induction h using Deduction.inducition_with_necOnly! with
   | hMaxm hp =>
     apply Deduction.maxm!;
     rcases hp with (hAxK | hAxL);
-    . obtain ⟨p, q, rfl⟩ := hAxK; simp [Formula.subst₂];
-    . obtain ⟨p, q, rfl⟩ := hAxL; simp [Formula.subst₂];
+    . obtain ⟨p, q, rfl⟩ := hAxK; simp [Formula.subst];
+    . obtain ⟨p, q, rfl⟩ := hAxL; simp [Formula.subst];
   | hMdp ihpq ihp =>
-    simp only [Formula.subst₂] at ihpq ihp;
+    simp only [Formula.subst] at ihpq ihp;
     exact ihpq ⨀ ihp;
   | hNec ih =>
-    simp only [Formula.subst₂];
+    simp only [Formula.subst];
     exact System.nec! ih;
   | _ =>
-    simp only [Formula.subst₂];
+    simp only [Formula.subst];
     trivial;
+
+lemma KH_deduct_substitution {p : Formula α} (a : α) (q : Formula α) : 𝐊𝐇 ⊢! p → 𝐊𝐇 ⊢! (p.subst a q) := by
+  intro h;
+  induction h using Deduction.inducition_with_necOnly! with
+  | hMaxm hp =>
+    apply Deduction.maxm!;
+    rcases hp with (hAxK | hAxH);
+    . obtain ⟨p, q, rfl⟩ := hAxK; simp [Formula.subst];
+    . obtain ⟨p, q, rfl⟩ := hAxH; simp [Formula.subst]; rfl;
+  | hMdp ihpq ihp => simp only [Formula.subst] at ihpq ihp; exact ihpq ⨀ ihp;
+  | hNec ih => simp only [Formula.subst]; exact System.nec! ih;
+  | _ => simp only [Formula.subst]; trivial;
 
 namespace Kripke
 
@@ -89,14 +58,6 @@ open Formula Formula.Kripke
 
 variable {a : α} {F : Kripke.Frame}
 
-/-
-lemma valid_H_of_valid_L {F : Kripke.Frame} : F# ⊧* (𝗟 : AxiomSet α) → F# ⊧* (𝗛 : AxiomSet α) := by
-  simp [Axioms.L, Axioms.H];
-  intro h p V x hx;
-  have : Satisfies ⟨F, V⟩ x (□(□p ⟶ p)) := by intro y Rxy; exact hx Rxy |>.1;
-  exact @h p V x this;
--/
-
 lemma valid_H_of_valid_L : F# ⊧ Axioms.L (atom a) → F# ⊧ Axioms.H (atom a) := by
   simp [Axioms.L, Axioms.H];
   intro h V x hx;
@@ -104,7 +65,7 @@ lemma valid_H_of_valid_L : F# ⊧ Axioms.L (atom a) → F# ⊧ Axioms.H (atom a)
   exact @h V x this;
 
 
-lemma valid_L_of_valid_H {a : α} {F : Kripke.Frame} : F# ⊧ Axioms.H (atom a) → F# ⊧ Axioms.L (atom a) := by
+lemma valid_L_of_valid_H : F# ⊧ Axioms.H (atom a) → F# ⊧ Axioms.L (atom a) := by
   simp [Axioms.L, Axioms.H];
   intro hH V x hx;
 
@@ -116,17 +77,18 @@ lemma valid_L_of_valid_H {a : α} {F : Kripke.Frame} : F# ⊧ Axioms.H (atom a) 
   have h₁ : Satisfies M' x (□(□a ⟷ a)) := by
     intro y Rxy;
     have : Satisfies M' y a ↔ Satisfies M' y (□a) := calc
-      _ ↔ ∀ n : ℕ, Satisfies M y (□^[n] a) := by simp [Satisfies];
-      _ ↔ ∀ n : ℕ, Satisfies M y (□^[(n + 1)]a) := by
+      _ ↔ ∀ n, Satisfies M y (□^[n] a) := by simp [Satisfies];
+      _ ↔ ∀ n, Satisfies M y (□^[(n + 1)]a) := by
         constructor;
         . intro h n; apply h;
         . intro h n;
-          have h₁ : Satisfies M y (□atom a ⟶ atom a) := @hx y Rxy;
-          have h₂ : Satisfies M y ((□atom a ⟶ atom a).subst₂ a (□^[n]atom a)) := Satisfies.subst_closed (a := a) (t := (□^[n](atom a))) h₁;
-          simp [Formula.subst₂] at h₂;
-          apply h₂;
-          aesop;
-      _ ↔ ∀ n : ℕ, ∀ z, y ≺ z → Satisfies M z (□^[n] a) := by simp [Satisfies];
+          have h₁ : Satisfies M y (□□^[n](atom a) ⟶ □^[n](atom a)) := by
+            induction n with
+            | zero => apply hx Rxy;
+            | succ n => intro _; apply h;
+          apply h₁;
+          simpa using h n;
+      _ ↔ ∀ n, ∀ z, y ≺ z → Satisfies M z (□^[n] a) := by simp [Satisfies];
       _ ↔ ∀ z, y ≺ z → ∀ n : ℕ, Satisfies M z (□^[n]a) := by aesop;
       _ ↔ ∀ z, y ≺ z → Satisfies M' z (atom a) := by simp [Satisfies];
       _ ↔ Satisfies M' y (□(atom a)) := by simp [Satisfies];
